State is so much more complicated!

state/TargetLang.fst
@@ -89,44 +89,37 @@ instance target_lang_ref (t:Type) {| c:target_lang t |} : target_lang (ref t) = 
 }
 
 let pre_tgt_arrow
-  (#tleaked:Type) (leaked:tleaked) {| tgts:target_lang tleaked |} 
+  (leaked:tfootprint)
   (#t1:Type) (x:t1) {| tgtx:target_lang t1 |}
   (h0:heap) =
-  dcontains (leaked, x) h0
+  dcontains x h0
 
 let post_tgt_arrow
-  (#tleaked:Type) (leaked:tleaked) {| tgts:target_lang tleaked |} 
+  (leaked:tfootprint)
   (#t1:Type) (x:t1) {| tgtx:target_lang t1 |}
   (#t2:t1 -> Type) {| tgtr : (x:t1 -> target_lang (t2 x)) |}
-  (h0:heap) (r:t2 x) (hf:heap) =
-  let fp0 = tgts.footprint leaked h0 in
-  let fpf = tgts.footprint leaked hf in
-  modifies fp0 h0 hf /\ 
-  equal_dom h0 hf /\ 
-  ((tgtr x).footprint r hf) ⊆ fp0 /\ 
-  fpf ⊆ fp0 /\ 
-  tgts.dcontains leaked hf /\ 
-  ((tgtr x).dcontains r hf)
+  (h0:heap) (r:t2 x) (h1:heap) =
+  let leaked = leaked ⊎ tgtx.footprint x h0 in
+  modifies leaked h0 h1 /\ 
+  equal_dom h0 h1 /\ 
+  ((tgtr x).footprint r h1) ⊆ leaked /\ 
+  ((tgtr x).dcontains r h1)
 
 unfold let mk_tgt_arrow  
   (t1:Type)
   {| tgt_t1: target_lang t1 |}
   (t2:t1 -> Type) 
-  (#tleaked:Type)
-  (leaked:tleaked)
-  {| tgt_leaked:target_lang tleaked |}
+  (leaked:tfootprint)
   {| c2 : (x:t1 -> target_lang (t2 x)) |}
 = x:t1 -> ST (t2 x) 
-    (requires (pre_tgt_arrow leaked #tgt_leaked x #tgt_t1))
-    (ensures (post_tgt_arrow leaked #tgt_leaked x #tgt_t1 #t2 #c2))
+    (requires (pre_tgt_arrow leaked x #tgt_t1))
+    (ensures (post_tgt_arrow leaked x #tgt_t1 #t2 #c2))
 
 instance target_lang_arrow 
   (t1:Type)
   {| target_lang t1 |}
-  (t2:t1 -> Type) 
-  (#tleaked:Type)
-  (leaked:tleaked)
-  {| target_lang tleaked |}
+  (t2:t1 -> Type)
+  (leaked:tfootprint)
   {| (x:t1 -> target_lang (t2 x)) |}
   : target_lang (mk_tgt_arrow t1 t2 leaked) = {
     footprint = (fun _ _ -> Set.empty); // <-- TODO: why no footprint for functions?
@@ -135,197 +128,67 @@ instance target_lang_arrow
     dcontains = (fun _ _ -> True);
   }
 
-
-(** ** Lemmas on target lang **)
-class target_lang_rels (a:Type) {| target_lang a |} (b:Type) {| target_lang b |} = {
-  footprint_footprint_after_write : r:ref a -> v:b -> h0:heap -> h1:heap -> fp_r:tfootprint -> 
-    Lemma (requires (
-      dcontains r h0 /\
-      dcontains v h0 /\
-      equal_dom h0 h1 /\
-      modifies !{r} h0 h1 /\
-      footprint r h1 ⊆ fp_r
-    ))
-    (ensures (footprint v h1 ⊆ footprint_after_write v h0 r fp_r))
-}
-
-instance target_lang_rels_unit (a:Type) {| target_lang a |} : target_lang_rels a unit = {
-  footprint_footprint_after_write = (fun _ _ _ _ _ -> ())
-}
-
-instance target_lang_rels_int (a:Type) {| target_lang a |} : target_lang_rels a int = {
-  footprint_footprint_after_write = (fun _ _ _ _ _ -> ())
-}
-
-instance target_lang_rels_pair
-  (a:Type) {| target_lang a |}
-  (b1:Type) {| target_lang b1 |}
-  (b2:Type) {| target_lang b2 |} 
-  {| target_lang_rels a b1 |}
-  {| target_lang_rels a b2 |}
-  : target_lang_rels a (b1 * b2) = {
-  footprint_footprint_after_write = (fun r (v1, v2) h0 h1 fp_r ->
-    footprint_footprint_after_write r v1 h0 h1 fp_r;
-    footprint_footprint_after_write r v2 h0 h1 fp_r
-  )
-}
-
-instance target_lang_rels_sums
-  (a:Type) {| target_lang a |}
-  (b1:Type) {| target_lang b1 |}
-  (b2:Type) {| target_lang b2 |} 
-  {| target_lang_rels a b1 |}
-  {| target_lang_rels a b2 |}
-  : target_lang_rels a (either b1 b2) = {
-  footprint_footprint_after_write = (fun r v h0 h1 fp_r ->
-    match v with
-    | Inl v1 -> footprint_footprint_after_write r v1 h0 h1 fp_r
-    | Inr v2 -> footprint_footprint_after_write r v2 h0 h1 fp_r
-  )
-}
-
-instance target_lang_rels_refs (a:Type) (b:Type) (#_:squash (a =!= b)) {| target_lang a |} {| target_lang b |} {| c1:target_lang_rels a b |}  : target_lang_rels a (ref b) = {
-  footprint_footprint_after_write = (fun r (v:ref b) h0 h1 fp_r ->
-    lemma_distinct_addrs_distinct_types h0 r v;
-    c1.footprint_footprint_after_write r (sel h0 v) h0 h1 fp_r;
-    assert ((!{v} ⊎ (footprint (sel h1 v) h1)) ⊆ !{v} ⊎ footprint_after_write (sel h0 v) h0 r fp_r);
-    lemma_modifies_and_equal_dom_sel_diff_addr !{r} h0 h1 v;
-    assert (sel h0 v == sel h1 v);
-    assert (footprint v h1 ⊆ footprint_after_write v h0 r fp_r)
-  )
-}
-
-instance target_lang_rels_refs' (a:Type) {| target_lang a |} {| c1:target_lang_rels a a |} : target_lang_rels a (ref a) = {
-  footprint_footprint_after_write = (fun r (v:ref a) h0 h1 fp_r ->
-    if compare_addrs v r then begin
-      lemma_sel_same_addr h0 v r;
-      assert ((!{v} ⊎ (footprint (sel h1 v) h1)) ⊆ (!{v} ⊎ fp_r));
-      assert (footprint r h1 ⊆ fp_r);
-      assert (footprint v h1 ⊆ footprint_after_write v h0 r fp_r)
-    end else begin
-      c1.footprint_footprint_after_write r (sel h0 v) h0 h1 fp_r;
-      assert ((!{v} ⊎ (footprint (sel h1 v) h1)) ⊆ !{v} ⊎ footprint_after_write (sel h0 v) h0 r fp_r);
-      lemma_modifies_and_equal_dom_sel_diff_addr !{r} h0 h1 v;
-      assert (sel h0 v == sel h1 v);
-      assert (footprint v h1 ⊆ footprint_after_write v h0 r fp_r)
-    end
-  )
-}
-
-instance target_lang_rels_arrow
-  (a:Type) {| target_lang a |}
-  (t1:Type) {| target_lang t1 |}
-  (t2:t1 -> Type) {| (x:t1 -> target_lang (t2 x)) |}
-  (#tleaked:Type)
-  (leaked:tleaked)
-  {| target_lang tleaked |} :
-  target_lang_rels a (mk_tgt_arrow t1 t2 leaked) = {
-    footprint_footprint_after_write = (fun _ _ _ _ _ -> ())
-  }
-
-let stable_footprint_v (#t:Type) {| target_lang t |} (* {| target_lang_rels t t |} *) (r:ref t) (v:t) (h0 h1:heap) :
-  Lemma
-    (requires (
-      dcontains r h0 /\
-      dcontains v h0 /\
-      equal_dom h0 h1 /\
-
-      modifies !{r} h0 h1 /\
-      sel h1 r == v 
-    ))
-    (ensures (footprint v h1 ⊆ footprint v h0))
-= // assume (!{r} `Set.disjoint` footprint v h0);
-  assume (!{r} ⊆ footprint v h0); // TODO: regression here after removing law1.
-  let fpr = !{r} ⊎ (footprint v h0) in
-  footprint_after_write_law v h0 r fpr;
-  assert (footprint_after_write v h0 r fpr ⊆ fpr ⊎ fpr);
-  assert (footprint_after_write v h0 r fpr ⊆ fpr);
-  assume (footprint r h1 ⊆ fpr);
-  admit ();
-  // footprint_footprint_after_write r v h0 h1 fpr;
-  assert (footprint v h1 ⊆ footprint_after_write v h0 r fpr)
-
-let footprint_r_after_write 
-  (#tleaked:Type) {| target_lang tleaked |} (leaked:tleaked)
-  (#t:Type) {| target_lang t |} (* {| target_lang_rels t tleaked |}*)
-  (r:ref t) (v:t)
-  (fp:Set.set nat)
-  (h0 h1:heap)
-  : Lemma
-  (requires (
-    equal_dom h0 h1 /\
-    dcontains leaked h0 /\
-    dcontains r h0 /\
-    modifies !{r} h0 h1 /\
-    sel h1 r == v /\
-    footprint leaked h0 ⊆ fp /\
-
-    !{r} ⊆ fp /\
-    footprint v h0 ⊆ fp
-  ))
-  (ensures (footprint leaked h1 ⊆ (fp ⊎ footprint r h1)))
-= footprint_after_write_law leaked h0 r (footprint r h1);
-  assert (footprint_after_write leaked h0 r (footprint r h1) ⊆ footprint leaked h0 ⊎ footprint r h1);
-  assert (footprint_after_write leaked h0 r (footprint r h1) ⊆ fp ⊎ footprint r h1);
-  admit ();
-  // footprint_footprint_after_write r leaked h0 h1 (footprint r h1);
-  assert (footprint leaked h1 ⊆ footprint_after_write leaked h0 r (footprint r h1))
-
-let equal_dom_preserves_dcontains (#t:Type) {| target_lang t |} (x:t) (h0 h1:heap) : Lemma
-  (requires (equal_dom h0 h1 /\ dcontains x h0))
-  (ensures (dcontains x h1)) = admit ()
-
-
-
-
-
 open STLC
 
+(** TODO:
+  let f : x:ref t   -> unit -> unit
+                    ^       ^
+                    |       |
+                    |       here x can have a different footprint, thus it is leaked again. 
+                    |       also, anything that was in x, could have a different footprint, thus it is leaked.
+                    the entire footprint of x is leaked
+**)
+
 (** *** Elaboration of types to F* *)
-let rec _elab_typ (t:typ) (#tleaked:Type) (leaked:tleaked) {| c_leaked:target_lang tleaked |} : tt:Type & target_lang tt =
+let rec _elab_typ (t:typ) (leaked:tfootprint) : tt:Type & target_lang tt =
   match t with
   | TArr t1 t2 -> begin
-    let tt1 = _elab_typ t1 #tleaked leaked #c_leaked in
-    let tt2 (x:dfst tt1) = _elab_typ t2 #(tleaked * dfst tt1) (leaked, x) #(target_lang_pair tleaked (dfst tt1) #c_leaked #(dsnd tt1)) in
-    (| mk_tgt_arrow      (dfst tt1) #(dsnd tt1) (fun x -> dfst (tt2 x)) leaked #c_leaked #(fun x -> dsnd (tt2 x)),
-       target_lang_arrow (dfst tt1) #(dsnd tt1) (fun x -> dfst (tt2 x)) leaked #c_leaked #(fun x -> dsnd (tt2 x))
+    let tt1 = _elab_typ t1 leaked in
+    let tt2 (x:dfst tt1) = _elab_typ t2 leaked in (* TODO: <-- leaked has to be extend with the footprint of x at this point *)
+    (| mk_tgt_arrow      (dfst tt1) #(dsnd tt1) (fun x -> dfst (tt2 x)) leaked #(fun x -> dsnd (tt2 x)),
+       target_lang_arrow (dfst tt1) #(dsnd tt1) (fun x -> dfst (tt2 x)) leaked #(fun x -> dsnd (tt2 x))
     |)
   end 
   | TUnit -> (| unit, target_lang_unit |)
   | TNat -> (| int, target_lang_int |)
   | TSum t1 t2 ->
-    let (| tt1, c_tt1 |) = _elab_typ t1 leaked #c_leaked in
-    let (| tt2, c_tt2 |) = _elab_typ t2 leaked #c_leaked in
+    let (| tt1, c_tt1 |) = _elab_typ t1 leaked in
+    let (| tt2, c_tt2 |) = _elab_typ t2 leaked in
     (| either tt1 tt2, target_lang_sum tt1 tt2 #c_tt1 #c_tt2 |)
   | TPair t1 t2 ->
-    let (| tt1, c_tt1 |) = _elab_typ t1 leaked #c_leaked in
-    let (| tt2, c_tt2 |) = _elab_typ t2 leaked #c_leaked in
+    let (| tt1, c_tt1 |) = _elab_typ t1 leaked in
+    let (| tt2, c_tt2 |) = _elab_typ t2 leaked in
     (| (tt1 * tt2), target_lang_pair tt1 tt2 #c_tt1 #c_tt2 |)
   | TRef t ->
-    let (| tt, c_tt |) = _elab_typ t leaked #c_leaked in
+    let (| tt, c_tt |) = _elab_typ t leaked in
     (| ref tt, target_lang_ref tt #c_tt |)
 
-let elab_typ (t:typ) (#tleaked:Type) (leaked:tleaked) {| c_leaked : target_lang tleaked |} : Type =
-  dfst (_elab_typ t leaked #c_leaked)
+let elab_typ (t:typ) (leaked:tfootprint) : Type =
+  dfst (_elab_typ t leaked)
 
-let elab_typ_tgt (t:typ) (#tleaked:Type) (leaked:tleaked) {| c_leaked : target_lang tleaked |} : target_lang (elab_typ t leaked)=
-  dsnd (_elab_typ t leaked #c_leaked)
+let elab_typ_tgt (t:typ) (leaked:tfootprint) : target_lang (elab_typ t leaked)=
+  dsnd (_elab_typ t leaked)
 
-let elab_typ' (t:typ) (#tleaked:typ) (leaked:dfst (_elab_typ tleaked ())) : Type =
-  let (| ty, c_leaked |) = _elab_typ tleaked () in
-  elab_typ t #ty leaked #c_leaked
+// let elab_typ' (t:typ) (#tleaked:typ) (leaked:dfst (_elab_typ tleaked ())) : Type =
+//   let (| ty, c_leaked |) = _elab_typ tleaked () in
+//   elab_typ t #ty leaked
 
-let elab_typ_tgt' (t:typ) (#tleaked:typ) (leaked:dfst (_elab_typ tleaked ())) : target_lang (elab_typ' t leaked)=
-  let (| ty, c_leaked |) = _elab_typ tleaked () in
-  elab_typ_tgt t #ty leaked #c_leaked
+// let elab_typ_tgt' (t:typ) (#tleaked:typ) (leaked:dfst (_elab_typ tleaked ())) : target_lang (elab_typ' t leaked)=
+//   let (| ty, c_leaked |) = _elab_typ tleaked () in
+//   elab_typ_tgt t #ty leaked #c_leaked
 
-// val elab_typ_test1 : elab_typ (TArr (TRef (TRef TNat)) (TArr (TRef TNat) TUnit))
-// let elab_typ_test1 (x:ref (ref int)) (y:ref int) =
-//   let ix = !x in
-//   ix := !ix + 1;
-//   x := y;
-//   y := !y + 5;
-//   ()
+val elab_typ_test0 : elab_typ (TArr (TRef TNat) TUnit) Set.empty
+let elab_typ_test0 (y:ref int) =
+  y := !y + 5;
+  ()
+
+val elab_typ_test1 : elab_typ (TArr (TRef (TRef TNat)) (TArr (TRef TNat) TUnit)) Set.empty
+let elab_typ_test1 (x:ref (ref int)) (y:ref int) =
+  let ix = !x in
+  ix := !ix + 1;
+  x := y;
+  y := !y + 5;
+  ()
 
 // val elab_typ_test2 : elab_typ (TArr TUnit (TRef TNat))
 // let elab_typ_test2 () = alloc 0
@@ -372,131 +235,16 @@ let vextend #t (x:elab_typ t ()) (#g:context) (ve:vcontext g) : vcontext (extend
 // let rec fnrec (#a:Type) (n:nat) (acc:a) (iter:a -> a): Tot a =
 //   if n = 0 then acc else fnrec (n-1) (iter acc) iter
 
-
-val elab_apply_arrow :
-  t1:typ ->
-  t2:typ ->
-  #tleaked:Type ->
-  leaked:tleaked ->
-  {| c_leaked: target_lang tleaked |} -> 
-  f:elab_typ (TArr t1 t2) leaked #c_leaked ->
-  (let tt1 = _elab_typ t1 leaked #c_leaked in
-   let tt2 (x:(dfst tt1)) = _elab_typ t2 (leaked, x) #(target_lang_pair tleaked (dfst tt1) #c_leaked #(dsnd tt1)) in
-   mk_tgt_arrow (dfst tt1) #(dsnd tt1) (fun x -> dfst (tt2 x)) leaked #c_leaked #(fun x -> dsnd (tt2 x)))
-let elab_apply_arrow t1 t2 #tleaked leaked #c_leaked f x = f x
-
-let rec elab_exp 
-  (#g:context)
-  (#e:exp) 
-  (#t:typ)
-  (tyj:typing g e t)
-  (ve:vcontext g)
-  (#tleaked:typ)
-  (leaked:elab_typ tleaked ())
-  : ST (elab_typ' t leaked) 
-     (requires (pre_tgt_arrow leaked #(elab_typ_tgt tleaked ()) ()))
-     (ensures (post_tgt_arrow leaked #(elab_typ_tgt tleaked ()) () #_ #(fun _ -> elab_typ' t leaked) #(fun _ -> elab_typ_tgt' t leaked)))
-     (decreases e) =
-  let tgt_leaked = elab_typ_tgt tleaked () in
-  let h0 = gst_get () in
-  let fp0 = tgt_leaked.footprint leaked h0 in
-  match tyj with
-  | TyUnit -> ()
-  | TyZero -> 0
-  | TyReadRef #_ #_ #t tyj_e -> begin
-    let r : ref (elab_typ' t leaked) = elab_exp tyj_e ve leaked in
-    read r
-  end
-  | TyWriteRef #_ #_ #_ #t tyj_ref tyj_v -> begin
-    let r : ref (elab_typ' t leaked) = elab_exp tyj_ref ve leaked in // <-- this is effectful and modifies fp
-      let h1 = gst_get () in
-      let fp1 = tgt_leaked.footprint leaked h1 in
-      let tgt_r = elab_typ_tgt' (TRef t) leaked in
-      
-      assert (tgt_r.dcontains r h1);
-      
-    let v : elab_typ' t leaked = elab_exp tyj_v ve leaked in // this is effectul and modifies fp
-      let h2 = gst_get () in
-      let fp2 = tgt_leaked.footprint leaked h2 in
-      let tgt_v = elab_typ_tgt' t leaked in
-
-    write r v;
-      let h3 = gst_get () in
-      let fp3 = tgt_leaked.footprint leaked h3 in
-      let fp_r = tgt_r.footprint r in
-      let fp_v = tgt_v.footprint v in
-      assert (tgt_v.footprint v h2 ⊆ fp1);
-      
-      // assert (fp2 ⊆ fp1 ⊆ fp0);
-      assert (tgt_r.footprint r h1 ⊆ fp0);
-      equal_dom_preserves_dcontains r h1 h2;
-      equal_dom_preserves_dcontains leaked h1 h2;
-      footprint_r_after_write leaked r v fp0 h2 h3;
-      assert (fp3 ⊆ fp0 ⊎ fp_r h3);
-      // assert ((fp2 `subtract` fp_r h2) ⊆ fp0);
-      assert (fp_r h3 `Set.equal` !{r} ⊎ fp_v h3);
-      stable_footprint_v r v h2 h3;
-      assert (fp_v h3 ⊆ fp_v h2);
-      assert (!{r} ⊆ fp0 /\ fp_v h2 ⊆ fp0 /\ fp_r h3 ⊆ fp0);
-
-      // post
-      assert (fp3 ⊆ fp0);
-      equal_dom_preserves_dcontains leaked h2 h3;
-      assert (tgt_leaked.dcontains leaked h3);
-    ()
-  end
-  | _ -> admit ()
-
-  // | TyAllocRef #_ #_ #t tyj_e -> begin
-  //   let v : elab_typ t = elab_exp tyj_e ve leaked #sfp in
-  //   let r = alloc v in
-  //   r
-  // end
-
-  (**
-  | TySucc hs ->
-    1 + (elab_exp hs ve)
-  | TyNRec h1 h2 h3 -> admit ()
-    // let v1 = elab_exp h1 ve in
-    // let v2 : elab_typ t = elab_exp h2 ve in
-    // let v3 : elab_typ (TArr t t) = elab_exp h3 ve in
-    // fnrec #(elab_typ t) v1 v2 v3
-  | TyInl #_ #_ #t1 #t2 h1 ->
-    let v = elab_exp h1 ve in
-    Inl #(elab_typ t1) #(elab_typ t2) v
-  | TyInr #_ #_ #t1 #t2 h1 ->
-    let v = elab_exp h1 ve in
-    Inr #(elab_typ t1) #(elab_typ t2) v
-  | TyCaseSum h1 h2 h3 ->
-    let v1 = elab_exp h1 ve in
-    let v2 = elab_exp h2 ve in
-    let v3 = elab_exp h3 ve in
-    (match v1 with | Inl x -> v2 x | Inr y -> v3 y)
-  | TyCaseNat h1 h2 h3 ->
-    let v1 = elab_exp h1 ve in
-    let v2 = elab_exp h2 ve in
-    let v3 = elab_exp h3 ve in
-    (match v1 with | 0 -> v2 () | _ -> v3 (v1-1))
-  | TyVar x -> ve x
-  | TyAbs t1 #_ #t2 h1 -> admit ()
-    // assert (t == TArr t1 t2);
-    // let w : elab_typ t1 -> Tot (elab_typ t2) =
-    // (fun x -> elab_exp h1 (vextend x ve)) in
-    // cast_TArr w
-  | TyApp #_ #_ #_ #t1 #t2 h1 h2 ->
-    assert ((elab_typ t) == (elab_typ t2));
-    (* TODO: Should we change the order here, first evaluate argument? *)
-    let v1 : elab_typ (TArr t1 t2) = elab_exp h1 ve in
-    let v2 : elab_typ t1 = elab_exp h2 ve in
-    v1 v2
-  | TyFst #_ #_ #t1 #t2 h1 ->
-    let v = elab_exp h1 ve in
-    fst #(elab_typ t1) #(elab_typ t2) v
-  | TySnd #_ #_ #t1 #t2 h1 ->
-    let v = elab_exp h1 ve in
-    snd #(elab_typ t1) #(elab_typ t2) v
-  | TyPair h1 h2 ->
-    let v1 = elab_exp h1 ve in
-    let v2 = elab_exp h2 ve in
-    (v1, v2)
-**)
+// let rec elab_exp 
+//   (#g:context)
+//   (#e:exp) 
+//   (#t:typ)
+//   (tyj:typing g e t)
+//   (ve:vcontext g)
+//   (#tleaked:typ)
+//   (leaked:elab_typ tleaked ())
+//   : ST (elab_typ' t leaked) 
+//      (requires (pre_tgt_arrow leaked #(elab_typ_tgt tleaked ()) ()))
+//      (ensures (post_tgt_arrow leaked #(elab_typ_tgt tleaked ()) () #_ #(fun _ -> elab_typ' t leaked) #(fun _ -> elab_typ_tgt' t leaked)))
+//      (decreases e) =
+//   admit ()
